Sealing up exception monad and axiomatizing some PureExecs for it

src/goose_lang/exception.v
@@ -1,5 +1,11 @@
 From Perennial.goose_lang Require Export notation.
 
+(* Q: Can we get by while keeping `do_return` etc. as sealed? *)
+(* Q: what about using modules for sealing? A: might make it impossible to
+   unfold, which might actually be useful.
+  Q: what about using modules for hiding everything except for a few exported
+     defns? So the default is to not export, and anything exported has to
+     explicitly marked. *)
 Section defn.
 
 Context `{ext_ty: ext_types}.
@@ -7,27 +13,36 @@ Context `{!ffi_syntax}.
 Local Coercion Var' s: expr := Var s.
 
 (* "Exception" monad *)
-Definition do_execute : val :=
+Local Definition do_execute_def : val :=
   λ: "v", (#(str "execute"), Var "v")
 .
 
+Program Definition do_execute := unseal (_:seal (@do_execute_def)). Obligation 1. by eexists. Qed.
+Definition do_execute_unseal : do_execute = _ := seal_eq _.
+
 (* Handle "execute" computations by dropping the final value and running the
    next sequential computation. *)
-Definition exception_seq : val :=
+Local Definition exception_seq_def : val :=
   λ: "s2" "s1",
     if: (Fst "s1") = #(str "execute") then
       "s2" #()
     else
       "s1"
 .
+Program Definition exception_seq := unseal (_:seal (@exception_seq_def)). Obligation 1. by eexists. Qed.
+Definition exception_seq_unseal : exception_seq = _ := seal_eq _.
 
-Definition do_return : val :=
+Local Definition do_return_def : val :=
   λ: "v", (#(str "return"), Var "v")
 .
+Program Definition do_return := unseal (_:seal (@do_return_def)). Obligation 1. by eexists. Qed.
+Definition do_return_unseal : do_return = _ := seal_eq _.
 
-Definition exception_do : val :=
+Definition exception_do_def : val :=
   λ: "v", Snd "v"
 .
+Program Definition exception_do := unseal (_:seal (@exception_do_def)). Obligation 1. by eexists. Qed.
+Definition exception_do_unseal : exception_do = _ := seal_eq _.
 
 End defn.
 
